quote "method" to allow Eisbach using this keyword;

thys/Jinja/Common/TypeRel.thy
@@ -498,7 +498,7 @@ lemma sees_field_idemp:
 
 subsection "Functional lookup"
 
-definition method :: "'m prog \<Rightarrow> cname \<Rightarrow> mname \<Rightarrow> cname \<times> ty list \<times> ty \<times> 'm"
+definition "method" :: "'m prog \<Rightarrow> cname \<Rightarrow> mname \<Rightarrow> cname \<times> ty list \<times> ty \<times> 'm"
 where
   "method P C M  \<equiv>  THE (D,Ts,T,m). P \<turnstile> C sees M:Ts \<rightarrow> T = m in D"
 
