thys/JinjaThreads/Common/TypeRel.thy
@@ -495,7 +495,7 @@ qed
 
 subsection "Functional lookup"
 
-definition method :: "'m prog \<Rightarrow> cname \<Rightarrow> mname \<Rightarrow> cname \<times> ty list \<times> ty \<times> 'm option"
+definition "method" :: "'m prog \<Rightarrow> cname \<Rightarrow> mname \<Rightarrow> cname \<times> ty list \<times> ty \<times> 'm option"
 where "method P C M  \<equiv>  THE (D,Ts,T,m). P \<turnstile> C sees M:Ts \<rightarrow> T = m in D"
 
 definition field  :: "'m prog \<Rightarrow> cname \<Rightarrow> vname \<Rightarrow> cname \<times> ty \<times> fmod"
