thys/CoreC++/Decl.thy
@@ -13,7 +13,7 @@ theory Decl imports Expr begin
 type_synonym
   fdecl    = "vname \<times> ty"                        -- "field declaration"
 type_synonym
-  method = "ty list \<times> ty \<times> (vname list \<times> expr)"    -- {* arg.\ types, return type, params, body *}
+  "method" = "ty list \<times> ty \<times> (vname list \<times> expr)"    -- {* arg.\ types, return type, params, body *}
 type_synonym
   mdecl = "mname \<times> method"                         -- "method declaration"
 type_synonym
